src/program_logic/staged_invariant_alt.v
@@ -1,0 +1,303 @@
+From iris.algebra Require Import gmap auth agree gset coPset excl csum.
+From Perennial.base_logic.lib Require Export fancy_updates.
+From stdpp Require Export namespaces.
+From Perennial.base_logic.lib Require Import wsat invariants ae_invariants saved_prop.
+From iris.algebra Require Import gmap.
+From iris.proofmode Require Import tactics.
+From Perennial.program_logic Require Export step_fupd_extra crash_weakestpre ae_invariants_mutable later_res private_invariants.
+Set Default Proof Using "Type".
+Import uPred.
+
+Class stagedG (Σ : gFunctors) : Set := WsatG {
+  staging_saved_inG :> savedPropG Σ;
+  staging_auth_inG :> inG Σ (authR (optionUR (exclR (prodO gnameO gnameO))));
+  staging_shot_inG :> inG Σ (csumR (fracR) (agreeR unitO));
+}.
+
+Definition stagedΣ : gFunctors :=
+  #[GFunctor (csumR fracR (agreeR unitO)); GFunctor (authR (optionUR (exclR (prodO gnameO gnameO))));
+   savedPropΣ].
+
+Instance subG_stagedG {Σ} : subG stagedΣ Σ → stagedG Σ.
+Proof. solve_inG. Qed.
+
+Definition staged_pending `{stagedG Σ} (q: Qp) (γ: gname) : iProp Σ :=
+  own γ (Cinl q).
+Definition staged_done `{stagedG Σ} (γ: gname) : iProp Σ :=
+  own γ (Cinr (to_agree ())).
+
+(* This is the modality guarding the crash condition in a wpc *)
+Definition wpc_crash_modality `{!irisGS Λ Σ, !crashG Σ} E1 Φc :=
+  ((∀ g1 ns D κs,
+       let E2 :=  ⊤ ∖ D in
+       global_state_interp g1 ns D κs -∗ C -∗
+     ||={E1|E2,∅|∅}=> ||▷=>^(num_laters_per_step ns) ||={∅|∅,E1|E2}=> global_state_interp g1 ns D κs ∗ Φc))%I.
+
+Section def.
+Context `{IRISG: !irisGS Λ Σ}.
+Context `{!pri_invG IRISG}.
+Context `{!later_tokG IRISG}.
+Context `{!stagedG Σ}.
+
+Definition staged_inv_inner E1 E2 (γ γ': gname) (P: iProp Σ) : iProp Σ :=
+  ((∃ γprop_stored γprop_remainder Ps Pr,
+             own γ (● Excl' (γprop_stored, γprop_remainder)) ∗
+             saved_prop_own γprop_stored Ps ∗
+             saved_prop_own γprop_remainder Pr ∗
+             (later_tok ∗ ((Ps ∗ pri_inv_tok E2 ∗ □ (Ps -∗ wpc_crash_modality E1 (P ∗ Pr)))
+                ∨
+              (Ps ∗ □ (Ps -∗ C ==∗ P ∗ Pr)))
+              ∨
+             (Pr ∗ C ∗ staged_done γ'))))%I.
+
+
+Definition staged_inv E1 E2 (γ γ': gname) (P: iProp Σ) : iProp Σ :=
+  (pri_inv E2 (staged_inv_inner E1 E2 γ γ' P)).
+
+Definition staged_value E1 (Ps Pr: iProp Σ) P : iProp Σ :=
+  (∃ E2 γ γ' γprop γprop', own γ (◯ Excl' (γprop, γprop')) ∗ saved_prop_own γprop Ps ∗ saved_prop_own γprop' Pr ∗ later_tok ∗ pri_inv_tok E2 ∗ staged_inv E1 E2 γ γ' P)%I.
+
+End def.
+
+Section inv.
+Context `{IRISG: !irisGS Λ Σ}.
+Context `{!pri_invG IRISG}.
+Context `{!later_tokG IRISG}.
+Context `{!stagedG Σ}.
+Implicit Types i : positive.
+Implicit Types N : namespace.
+Implicit Types P Q R : iProp Σ.
+
+(* TODO: this is annoying but true *)
+(*
+Global Instance staged_contractive  E γ γ' : Contractive (staged_inv E γ γ').
+Proof.
+  rewrite /staged_inv=> n ?? ?.
+  rewrite pri_inv_full_eq /pri_inv_full_def.
+  f_equiv => ?.
+  rewrite pri_inv_eq /pri_inv_def.
+  do 4 f_equiv.
+Qed.
+
+Global Instance staged_ne N k E E' γ γ': NonExpansive (staged_inv N k E E' γ γ').
+Proof.
+  rewrite /staged_inv=> n ?? ?.
+  repeat (apply step_fupdN_ne || f_contractive || f_equiv); eauto using dist_le.
+Qed.
+
+Global Instance staged_proper N k E E' γ γ' : Proper ((⊣⊢) ==> (⊣⊢)) (staged_inv N k E E' γ γ').
+Proof. apply ne_proper, _. Qed.
+*)
+
+Global Instance staged_persistent E1 E2 γ γ' P : Persistent (staged_inv E1 E2 γ γ' P).
+Proof. rewrite /staged_inv. apply _. Qed.
+
+Lemma pending_done q γ: staged_pending q γ -∗ staged_done γ -∗ False.
+Proof.
+  rewrite /staged_pending/staged_done.
+  iIntros "H H'".
+  { by iDestruct (own_valid_2 with "H H'") as %?. }
+Qed.
+
+Lemma pending_upd_done γ: staged_pending 1%Qp γ ==∗ staged_done γ.
+Proof.
+  rewrite /staged_pending/staged_done.
+  iIntros "H". iMod (own_update with "H") as "$".
+  { by apply cmra_update_exclusive. }
+  done.
+Qed.
+
+Lemma pending_alloc:
+  ⊢ |==> ∃ γ, staged_pending 1 γ.
+Proof.
+  iApply (own_alloc (Cinl 1%Qp)).
+  { rewrite //=. }
+Qed.
+
+Lemma pending_split γ:
+  staged_pending 1 γ ⊢ staged_pending (1/2)%Qp γ ∗ staged_pending (1/2)%Qp γ.
+Proof. by rewrite /staged_pending -own_op -Cinl_op frac_op Qp_div_2. Qed.
+
+Lemma pending_split34 γ:
+  staged_pending 1 γ ⊢ staged_pending (3/4)%Qp γ ∗ staged_pending (1/4)%Qp γ.
+Proof. by rewrite /staged_pending -own_op -Cinl_op frac_op Qp_three_quarter_quarter. Qed.
+
+Lemma pending_join γ:
+ staged_pending (1/2)%Qp γ ∗ staged_pending (1/2)%Qp γ ⊢  staged_pending 1 γ.
+Proof. by rewrite /staged_pending -own_op -Cinl_op frac_op Qp_div_2. Qed.
+
+Lemma pending_join34 γ:
+ staged_pending (3/4)%Qp γ ∗ staged_pending (1/4)%Qp γ ⊢  staged_pending 1 γ.
+Proof. by rewrite /staged_pending -own_op -Cinl_op frac_op Qp_three_quarter_quarter. Qed.
+
+Lemma pending34_pending34 γ:
+ staged_pending (3/4)%Qp γ -∗ staged_pending (3/4)%Qp γ -∗ False.
+Proof.
+  rewrite /staged_pending.
+  iIntros "H H'".
+  { by iDestruct (own_valid_2 with "H H'") as %?. }
+Qed.
+
+Lemma pending_pending γ:
+ staged_pending 1%Qp γ -∗ staged_pending 1%Qp γ -∗ False.
+Proof.
+  rewrite /staged_pending.
+  iIntros "H H'".
+  { by iDestruct (own_valid_2 with "H H'") as %?. }
+Qed.
+
+(* TODO : *)
+(*
+Lemma staged_inv_iff E i γ γ' P Q :
+  ▷ □ (P ↔ Q) -∗
+  staged_inv E i γ γ' P -∗
+  staged_inv E i γ γ' Q.
+Proof.
+  iIntros "#HPQ". iApply inv_iff. iNext. iAlways. iSplit.
+  - iIntros "H". iDestruct "H" as (?? P0 P0') "(?&?&?&#HP0&Hcase)". iExists _, _, P0, P0'. iFrame.
+    iAlways. iIntros. iSpecialize ("HP0" with "[$] [$]").
+    iApply (step_fupdN_inner_wand' with "HP0"); eauto.
+    iIntros "(?&$)". by iApply "HPQ".
+  - iIntros "H". iDestruct "H" as (?? P0 P0') "(?&?&?&#HP0&Hcase)". iExists _, _, P0, P0'. iFrame.
+    iAlways. iIntros. iSpecialize ("HP0" with "[$] [$]").
+    iApply (step_fupdN_inner_wand' with "HP0"); eauto.
+    iIntros "(?&$)". by iApply "HPQ".
+Qed.
+*)
+
+Lemma wpc0_pri_inv_tok_res s k D E1 e Φ Φc :
+  (∀ E', (⌜ E' ## D ⌝ ∧ pri_inv_tok E') -∗
+          ||={E1|⊤∖D, E1|⊤∖D}=> wpc0 s k D E1 e Φ Φc) -∗
+  wpc0 s k D E1 e Φ Φc.
+Proof.
+  iIntros "H".
+  iEval (rewrite wpc0_unfold).
+  rewrite /wpc_pre.
+  iSplit.
+  {
+    destruct (to_val e) eqn:Heq_val.
+    - iIntros (q g1 ns κs) "Hg HNC".
+      iMod (pri_inv_tok_alloc with "[$]") as (Einv Hdisj) "(Hitok&Hg)".
+      iSpecialize ("H" with "[$Hitok //]").
+      rewrite wpc0_unfold/ wpc_pre. rewrite Heq_val.
+      iMod "H" as "(H&_)". by iMod ("H" with "[$] [$]") as "$".
+    - iIntros.
+      iMod (pri_inv_tok_alloc with "[$]") as (Einv Hdisj) "(Hitok&Hg)".
+      iSpecialize ("H" with "[$Hitok //]").
+      rewrite wpc0_unfold/ wpc_pre. rewrite Heq_val.
+      iMod "H" as "(H&_)". by iMod ("H" with "[$] [$] [$]") as "$".
+  }
+  iIntros.
+  iMod (pri_inv_tok_alloc with "[$]") as (Einv Hdisj) "(Hitok&Hg)".
+  iSpecialize ("H" with "[$Hitok //]").
+  rewrite wpc0_unfold/ wpc_pre.
+  iMod "H" as "(_&H)". by iMod ("H" with "[$] [$]") as "$".
+Qed.
+
+Existing Instances pri_inv_tok_timeless later_tok_timeless.
+
+Lemma wpc_staged_inv_init s k E e Φ Φc P Pc:
+  later_tok ∗
+  later_tok ∗
+  P ∗
+  □ (P -∗ Pc) ∗
+  (staged_value E P True Pc -∗ WPC e @ s; k; E {{ Φ }} {{ Φc }})
+  ⊢ WPC e @ s; k; E {{ Φ }} {{ Φc ∗ Pc }}.
+Proof.
+  iIntros "(Htok1&Htok2&HP&#Hwand&Hwp)".
+  rewrite wpc_eq /wpc_def. iIntros (D).
+  iApply wpc0_pri_inv_tok_res.
+  iIntros (Einv) "(%Hdisj&Hitok)".
+
+  (* Create the invariant *)
+
+  iMod (saved_prop_alloc P) as (γprop) "#Hsaved".
+  iMod (saved_prop_alloc True%I) as (γprop') "#Hsaved'".
+  iMod (own_alloc (● (Excl' (γprop, γprop')) ⋅ ◯ (Excl' (γprop, γprop')))) as (γ) "[H1 H2]".
+  { apply auth_both_valid_2; [econstructor | reflexivity]. }
+  iMod (pending_alloc) as (γ') "H".
+
+  iDestruct (pri_inv_tok_infinite with "Hitok") as %Hinf.
+  iMod (pri_inv_alloc Einv _ _ (staged_inv_inner E Einv γ γ' Pc) with "[HP H1 Htok2]") as "#Hpri_inv"; auto.
+  { iNext. rewrite /staged_inv_inner. iExists _, _, P, True%I. iFrame "∗ #".
+    iLeft. iFrame. iRight.
+    iModIntro. iIntros "HP HC". iModIntro. iDestruct ("Hwand" with "[$]") as "$"; eauto.
+  }
+
+  (* The inductive proof *)
+  iSpecialize ("Hwp" with "[Htok1 Hitok H2]").
+  { iExists _, _, _, _, _. iFrame "∗ #". }
+  iSpecialize ("Hwp" $! D).
+
+  iModIntro.
+  iLöb as "IH" forall (e).
+  rewrite ?wpc0_unfold. rewrite /wpc_pre.
+  iSplit; last first.
+  {
+    iDestruct "Hwp" as "(_&Hwp)".
+    iIntros (g ns κs) "Hg #HC".
+    iMod (pri_inv_acc with "Hpri_inv") as "(Hinner&Hclo)".
+    { set_solver. }
+    iDestruct "Hinner" as (????) "(Hown1&#Hsaved1&#Hsaved2&Hinner)".
+    iDestruct "Hinner" as "[(>Hltok&Hs)|Hbad]"; last first.
+    {
+      (* This case is impossible since we have the staged_pending token *)
+      iDestruct "Hbad" as "(_&_&>Hdone)".
+      iDestruct (pending_done with "[$] [$]") as %[].
+    }
+    iMod (later_tok_decr with "[$]") as (ns' Hle) "Hg".
+    iApply (step_fupd2N_inner_le).
+    { apply (num_laters_per_step_exp ns'). lia. }
+    simpl.
+    iMod (fupd2_mask_subseteq ∅ ∅) as "Hclo'"; try set_solver+.
+    iModIntro. iModIntro. iNext.
+    iMod "Hclo'".
+    iDestruct "Hs" as "[Hinuse|Hunused]".
+    {
+      iDestruct "Hinuse" as "(HPs&Hitok&#Hwand')".
+      iDestruct ("Hwand'" with "[$]") as "HPcr".
+      rewrite /wpc_crash_modality.
+      iApply step_fupd2N_inner_plus.
+      iMod (pri_inv_tok_disable with "[$]") as "Hg".
+      replace (⊤ ∖ D ∖ Einv) with (⊤ ∖ (Einv ∪ D)) by set_solver.
+      iSpecialize ("HPcr" with "[$] [$]").
+      iApply (step_fupd2N_inner_wand with "HPcr"); auto.
+      iIntros "(Hg&HPc&HPr)".
+      replace (⊤ ∖ (Einv ∪ D)) with (⊤ ∖ D ∖ Einv) by set_solver.
+      iMod (pri_inv_tok_enable with "[$Hg //]") as "(Hitok&Hg)".
+      iMod (pending_upd_done with "H") as "H".
+      iMod ("Hclo" with "[HPr Hitok Hown1 H]").
+      { iNext. iExists _, _, _, _. iFrame "∗ #". iRight. iFrame. }
+      iSpecialize ("Hwp" with "[$] [$]").
+      iApply step_fupd2N_inner_fupd.
+      iApply (step_fupd2N_inner_wand with "Hwp"); auto. iIntros "(Hg&$)". iFrame.
+      iApply (global_state_interp_le with "[$]"); eauto.
+      lia.
+    }
+    {
+      iDestruct "Hunused" as "(HPs&#Hwand')".
+      iMod ("Hwand'" with "[$] [$]") as "(HPc&HPr)".
+      iMod (pending_upd_done with "H") as "H".
+      iMod ("Hclo" with "[HPr Hown1 H]").
+      { iNext. iExists _, _, _, _. iFrame "∗ #". iRight. iFrame. }
+      iApply step_fupd2N_inner_plus.
+      iApply step_fupd2N_inner_later; auto. iNext.
+      iSpecialize ("Hwp" with "[$] [$]").
+      iApply step_fupd2N_inner_fupd.
+      iApply (step_fupd2N_inner_wand with "Hwp"); auto. iIntros "(Hg&$)". iFrame.
+      iApply (global_state_interp_le with "[$]"); eauto.
+      lia.
+    }
+  }
+  iDestruct "Hwp" as "(Hwp&_)".
+  destruct (to_val e).
+  { iIntros. iMod ("Hwp" with "[$] [$]"). eauto. }
+  iIntros.
+  iMod ("Hwp" with "[$] [$] [$]") as "Hwp".
+  iModIntro. simpl. iMod "Hwp". iModIntro.
+  iNext. iMod "Hwp". iModIntro. iApply (step_fupd2N_wand with "Hwp").
+  iIntros "($&Hwp)".
+  iIntros. iMod ("Hwp" with "[//]") as "($&$&Hwpc&$&$)". iModIntro. iApply ("IH" with "[$] [$]").
+Qed.
+
+End inv.
